recon/syntax.v
@@ -1,0 +1,554 @@
+Require Coq.extraction.Extraction.
+Require Import Ascii String Coq.Strings.Byte.
+From Coq Require Import Lists.List.
+Import ListNotations.
+Require Export ExtrOcamlChar.
+Extract Inductive bool => "bool" ["true" "false"].
+Extract Inductive string => "char list" [ "[]" "(::)" ].
+Extract Inductive list => "list" [ "[]" "(::)" ].
+Extraction Language OCaml.
+Load "../std".
+
+Inductive ty : Type :=
+| Bool
+| Arrow (ty1 ty2: ty)
+| TyVar: nat -> ty.
+Notation "t1 '|-->' t2" := (Arrow t1 t2) (at level 40).
+
+Inductive term : Type :=
+(*純粋λ計算*)
+| Var (n: nat)
+| Abs (name: string) (typ: ty) (t: term)
+| App (t1 t2: term)
+(*ぶーる*)
+| Tru
+| Fls
+| If (t1 t2 t3: term).
+
+Inductive value : term -> Prop :=
+| V_tru : value Tru
+| V_fls : value Fls
+| V_abs :forall typ name t1, value (Abs typ name t1).
+
+Definition context : Type := list ty.
+
+Definition eqb_string s1 s2:=
+  String.eqb s1 s2.
+
+Fixpoint getbinding (n : nat) (ctx: context) :=
+  match n with
+  | 0 =>
+    match ctx with
+    | [] => None
+    | t :: ctx' => Some t
+    end
+  | S n' =>
+    match ctx with
+    | [] => None
+    | x :: ctx' => getbinding n' ctx'
+    end
+  end.
+
+Definition isval t:=
+match t with
+| Tru => true
+| Fls => true
+| Abs _ _ _ => true
+| _ => false
+end.
+
+Fixpoint eqb_ty (T1 T2: ty) : bool :=
+  match (T1, T2) with
+  | (Bool, Bool) => true
+  | (T11 |--> T12, T21 |--> T22) =>
+    andb (eqb_ty T11 T21) (eqb_ty T12 T22)
+  | (TyVar n1, TyVar n2) => Nat.eqb n1 n2
+  | _ => false
+  end.
+
+Reserved Notation "ctx '|-' x '\in' t" (at level 40).
+Inductive has_type : context -> term -> ty -> Prop :=
+| T_True:
+    forall ctx,
+      ctx |- Tru \in Bool
+| T_False:
+    forall ctx,
+      ctx |- Fls \in Bool
+| T_If:
+    forall ctx t1 t2 t3 T',
+      ctx |- t1 \in Bool ->
+      ctx |- t2 \in T' ->
+      ctx |- t3 \in T' ->
+      ctx |- (If t1 t2 t3) \in T'
+| T_Var:
+    forall ctx n1 t,
+      getbinding n1 ctx = Some t ->
+      ctx |- (Var n1) \in t
+| T_Abs:
+    forall ctx x T1 t2 T2,
+      (T1 :: ctx) |- t2 \in T2 ->
+      ctx |- (Abs x T1 t2) \in (T1 |--> T2)
+| T_App:
+    forall ctx t1 T11 T12 t2,
+      ctx |- t1 \in (T11 |--> T12) ->
+      ctx |- t2 \in T11 ->
+      ctx |- App t1 t2 \in T12
+
+where " ctx '|-' x '\in' t " := (has_type ctx x t).
+
+
+Example type1:
+  [((Bool |--> Bool))] |- App (Var 0) (If Fls Tru Fls) \in Bool.
+Proof.
+  eapply T_App. apply T_Var. reflexivity.
+  apply T_If. apply T_False. apply T_True. apply T_False.
+Qed.
+
+Example type2:
+  [((Bool |--> Bool))] |- (Abs "x" Bool (App (Var 1) (If (Var 0) Fls (Var 0)))) \in (Bool |--> Bool).
+Proof.
+  apply T_Abs. eapply T_App. apply T_Var. reflexivity.
+  apply T_If. apply T_Var. reflexivity. apply T_False. apply T_Var. reflexivity.
+Qed.
+
+Lemma eq_type_refl : forall T,
+    eqb_ty T T = true.
+Proof.
+  induction T; simpl; auto. rewrite IHT1, IHT2; auto. apply Nat.eqb_refl.
+Qed.
+
+Lemma eqb_ty_eq : forall T1 T2,
+    eqb_ty T1 T2 = true <-> T1 = T2.
+Proof.
+  split; intros.
+  generalize dependent T2; induction T1; intros;
+    destruct T2; try solve_by_invert; auto.
+  simpl in H. apply andb_prop in H; destruct H.
+  apply IHT1_1 in H. apply IHT1_2 in H0; subst. reflexivity.
+
+  simpl in H. apply Nat.eqb_eq in H; subst. reflexivity.
+
+  subst. apply eq_type_refl.
+Qed.
+
+Fixpoint typeof ctx t : option ty :=
+  match t with
+  | Tru =>
+    (Some Bool)
+  | Fls =>
+    Some Bool
+  | If t1 t2 t3 =>
+    match typeof ctx t1 with
+    | Some Bool =>
+      match typeof ctx t2 with
+      | Some T2 =>
+        match typeof ctx t3 with
+        | Some T3 =>
+          if eqb_ty T2 T3 then
+            Some T2
+          else
+            None
+        | None => None
+        end
+      | None => None
+      end
+    | _ => None
+    end
+  | Var n =>
+    getbinding n ctx
+  | Abs x T1 t1 =>
+    match typeof (T1 :: ctx) t1 with
+    | Some T2 =>
+      Some (T1 |--> T2)
+    | None => None
+    end
+  | App t1 t2 =>
+    match typeof ctx t1 with
+    | Some (T11 |--> T12) =>
+      match typeof ctx t2 with
+      | Some T21 =>
+        if eqb_ty T11 T21 then
+          Some T12
+        else
+          None
+      | None => None
+      end
+    | _ => None
+    end
+  end.
+
+Lemma typeof_hasType : forall t ctx T,
+    has_type ctx t T <-> typeof ctx t = Some T.
+Proof.
+  split; intros.
+  -
+    induction H; simpl; auto.
+    +
+      rewrite IHhas_type1, IHhas_type2, IHhas_type3. clear.
+      rewrite eq_type_refl; reflexivity.
+    +
+      rewrite IHhas_type. reflexivity.
+    +
+      rewrite IHhas_type2, IHhas_type1. rewrite eq_type_refl; reflexivity.
+  -
+    generalize dependent T. generalize dependent ctx; induction t; intros; simpl; auto.
+    +
+      inversion H; subst; apply T_Var; simpl; auto.
+    +
+      inversion H; subst. destruct (typeof ((typ) :: ctx) t) eqn:IH. inversion H1; subst.
+      apply IHt in IH. apply T_Abs. apply IH. inversion H1.
+    +
+      simpl in H.
+      destruct (typeof ctx t1) eqn:IH1; try discriminate.
+      destruct t; try discriminate.
+      destruct (typeof ctx t2) eqn:IH2; try discriminate.
+      apply IHt1 in IH1. apply IHt2 in IH2.
+      destruct (eqb_ty t3 t) eqn:IH3; try discriminate. apply eqb_ty_eq in IH3; subst.
+      inversion H; subst. econstructor; eauto.
+    +
+      inversion H. apply T_True.
+    +
+      inversion H. apply T_False.
+    +
+      inversion H.
+      destruct (typeof ctx t1) eqn:IH1; try discriminate.
+      destruct t; try discriminate.
+      destruct (typeof ctx t2) eqn:IH2; try discriminate.
+      apply IHt1 in IH1. apply IHt2 in IH2.
+      destruct (typeof ctx t3) eqn:IH3; try discriminate. apply IHt3 in IH3.
+      destruct (eqb_ty t t0) eqn:IH4; try discriminate.
+      apply eqb_ty_eq in IH4; subst.
+      inversion H1; subst.
+      constructor; auto.
+Qed.
+
+
+Lemma leb_0_T : forall n,
+    Nat.leb 0 n = true.
+Proof.
+  induction n; auto.
+Qed.
+
+Fixpoint in_free t n :=
+  match t with
+  | Var n1 =>
+    if Nat.leb n n1 then
+      true
+    else
+      false
+  | Abs x T t1 =>
+    in_free t1 (S n)
+  | App t1 t2 =>
+    in_free t1 n || in_free t2 n
+  | Tru => false
+  | Fls => false
+  | If t1 t2 t3 =>
+    in_free t1 n || in_free t2 n || in_free t3 n
+  end.
+
+Notation closed t := (in_free t 0 = false).
+
+Lemma var_hastype_none : forall ctx,
+    getbinding (length ctx) ctx = None.
+Proof.
+  induction ctx; auto.
+Qed.
+
+Lemma var_hastype_none_succ : forall n ctx,
+    Nat.leb (length ctx) n = true ->
+    getbinding n ctx = None.
+Proof.
+  induction n; intros; auto.
+  destruct ctx; auto. simpl in H. inversion H.
+  destruct ctx. simpl. reflexivity.
+  simpl. apply IHn. apply Nat.leb_le. apply le_S_n. apply Nat.leb_le. apply H.
+Qed.
+
+Require Import Nat.
+Lemma closed_hastype : forall t T ctx,
+    ctx |- t \in T ->
+    in_free t (length ctx) = false.
+Proof.
+  induction t; intros; simpl; inversion H; subst; auto.
+  destruct leb eqn:IH; auto. rewrite var_hastype_none_succ in H2. inversion H2. apply IH.
+  apply IHt in H5. simpl in H5. apply H5.
+  apply IHt1 in H3. apply IHt2 in H5. rewrite H3, H5; reflexivity.
+  apply IHt1 in H4. apply IHt2 in H6. apply IHt3 in H7. rewrite H4, H6, H7; reflexivity.
+Qed.
+
+Lemma cosed_type_nil : forall t T,
+    [] |- t \in T ->
+    closed t.
+Proof.
+  intros. apply closed_hastype in H. simpl in H. apply H.
+Qed.
+
+Lemma appGetbind : forall ctx ctx' n,
+    getbinding (n + (length ctx)) (ctx ++ ctx') = getbinding n ctx'.
+Proof.
+  induction ctx; simpl; intros; auto.
+  rewrite <- plus_n_O; reflexivity.
+  rewrite <- plus_Snm_nSm. simpl. apply IHctx.
+Qed.
+
+Lemma length1_Some : forall n ctx ctx1 ctx2 T,
+    n < length ctx ->
+    getbinding n (ctx ++ ctx1) = Some T ->
+    getbinding n (ctx ++ ctx2) = Some T.
+Proof.
+  induction n; simpl; intros. destruct ctx. inversion H. simpl. simpl in H0. apply H0.
+  destruct ctx. inversion H. simpl. destruct ( (t :: ctx) ++ ctx1) eqn:IHH. inversion H0. inversion IHH; subst.
+  eapply IHn in H0. apply H0. simpl in H. apply lt_S_n in H. apply H.
+Qed.
+
+
+(**)
+Fixpoint shift (d k : nat) (t : term) : term :=
+match t with
+| Var x =>
+  Var (if leb d x then x + k else x)
+| Abs x T t' =>
+  Abs x T (shift (S d) k t')
+| App t1 t2 =>
+  App (shift d k t1) (shift d k t2)
+| Tru => Tru
+| Fls => Fls
+| If t1 t2 t3 =>
+  If (shift d k t1) (shift d k t2) (shift d k t3)
+end.
+
+Fixpoint subst (d : nat) (s t: term) : term :=
+match t with
+| Var x =>
+  if eqb d x then (*d == x*)
+    shift 0 d s
+  else if ltb d x then (*d < x*)
+         Var (pred x) else
+         Var x (*d > x*)
+| Abs x T t' => Abs x T (subst (S d) s t')
+| App t1 t2 => App (subst d s t1) (subst d s t2)
+| Tru => Tru
+| Fls => Fls
+| If t1 t2 t3 =>
+  If (subst d s t1) (subst d s t2) (subst d s t3)
+end.
+
+Fixpoint eval (t: term) :=
+  match t with
+  | If t1 t2 t3 =>
+    match t1 with
+    | Tru => Some t2
+    | Fls => Some t3
+    | _ => match eval t1 with
+          | Some t1' =>
+            Some (If t1' t2 t3)
+          | None => None
+          end
+    end
+  | App t1 t2 =>
+    if isval t1 then
+      if isval t2 then
+        match t1 with
+        | Abs _ _ t12 => Some (subst 0 t2 t12)
+        | _ => None
+        end
+      else
+        match eval t2 with
+        | Some t2' => Some (App t1 t2')
+        | None => None
+        end
+    else
+      match eval t1 with
+      | Some t1' => Some (App t1' t2)
+      | None => None
+      end
+  | _ => None
+  end.
+
+Reserved Notation " t '-->' t' " (at level 40).
+Inductive step :term -> term -> Prop :=
+| E_IfTrue : forall t2 t3,
+    If Tru t2 t3 --> t2
+| E_IfFalse : forall t2 t3,
+    If Fls t2 t3 --> t3
+| E_If : forall t1 t1' t2 t3,
+    t1 --> t1' ->
+    If t1 t2 t3 --> If t1' t2 t3
+| E_App1 : forall t1 t2 t1',
+    t1 --> t1' ->
+    App t1 t2 --> App t1' t2
+| E_App2 : forall v1 t2 t2',
+    value v1 ->
+    t2 --> t2' ->
+    App v1 t2 --> App v1 t2'
+| E_AppAbs : forall typ str t12 t2,
+    value t2 ->
+    App (Abs typ str t12) t2 --> subst 0 t2 t12
+
+  where " t '-->' t' " := (step t t').
+
+Lemma shift0 : forall t n,
+    shift n 0 t = t.
+Proof.
+  induction t; intros; simpl; eauto.
+  rewrite <- plus_n_O. destruct leb; reflexivity.
+
+  rewrite IHt; reflexivity.
+  rewrite IHt1, IHt2; reflexivity.
+  rewrite IHt1, IHt2, IHt3; reflexivity.
+Qed.
+
+Lemma E9_3_2 :  forall n T,
+    not (exists ctx,ctx |- App (Var n) (Var n) \in T).
+Proof.
+  intros; intro. inversion H.
+  inversion H0; subst. inversion H4. inversion H6; subst.
+  rewrite H9 in H3. inversion H3. apply eqb_ty_eq in H2.
+  generalize H2. clear. generalize dependent T.
+  induction T11; intros. inversion H2. inversion H2. apply andb_prop in H0. inversion H0.
+  apply IHT11_1 in H. apply H. inversion H2.
+Qed.
+
+Lemma T9_3_3 : forall t1 ctx T1 T2,
+    ctx |- t1 \in T1 ->
+    ctx |- t1 \in T2 ->
+    T1 = T2.
+Proof.
+  induction t1; intros.
+  -
+    inversion H; inversion H0; subst. rewrite H3 in H7. inversion H7; reflexivity.
+  -
+    inversion H; inversion H0; subst.
+    apply eqb_ty_eq. simpl; apply andb_true_intro; split; auto.
+    clear. induction typ; auto. simpl. apply andb_true_intro. split; auto.
+    apply eqb_ty_eq. reflexivity.
+    eapply IHt1 in H6; eauto. subst. rewrite eqb_ty_eq. reflexivity.
+  -
+    inversion H; inversion H0; subst.
+    apply IHt1_1 with (T2:= (T0 |--> T2)) in H4; auto.
+    inversion H4; reflexivity.
+  -
+    inversion H; inversion H0; subst; auto.
+  -
+    inversion H; inversion H0; subst; auto.
+  -
+    inversion H; inversion H0; subst; auto.
+    apply (IHt1_2 ctx T1 T2); auto.
+Qed.
+
+Lemma L9_3_4_bool : forall ctx v,
+    value v ->
+    ctx |- v \in Bool ->
+    v = Tru \/ v = Fls.
+Proof.
+  intros. inversion H0; subst. left; auto. right; auto.
+  inversion H. inversion H. inversion H.
+Qed.
+
+Lemma L9_3_4_Abs: forall ctx v T1 T2,
+    value v ->
+    ctx |- v \in (T1 |--> T2) ->
+    exists x t, v = Abs x T1 t.
+Proof.
+  intros. inversion H0; subst; try solve_by_invert.
+  exists x, t2. reflexivity.
+Qed.
+
+Theorem T9_3_5 : forall t T,
+    [] |- t \in T ->
+    value t \/ exists t', t --> t'.
+Proof.
+  induction t; simpl; intros.
+  -
+    inversion H; subst. destruct n; inversion H2.
+  -
+    left; apply V_abs.
+  -
+    right.
+    inversion H; subst.
+    generalize H3; intro. apply IHt1 in H3. destruct H3.
+    apply (L9_3_4_Abs [] t1) in H0; auto. inversion H0. inversion H2.
+    apply IHt2 in H5. inversion H5. rewrite H3.
+    exists (subst 0 t2 x0). apply E_AppAbs; auto.
+    inversion H4. exists (App t1 x1). apply E_App2; auto.
+    inversion H1. exists (App x t2); apply E_App1; auto.
+  -
+    left. apply V_tru.
+  -
+    left; apply V_fls.
+  -
+    inversion H; subst. right. generalize H4; intros; apply IHt1 in H4.
+    destruct H4. apply (L9_3_4_bool [] t1) in H1; auto. destruct H1; rewrite H1.
+    exists t2; apply E_IfTrue. exists t3; apply E_IfFalse. inversion H1.
+    exists (If x t2 t3); apply E_If; auto.
+Qed.
+
+Lemma shifting : forall t g g1 g2 T,
+  (g1 ++ g) |- t \in T ->
+  (g1 ++ g2 ++ g) |- (shift (length g1) (length g2) t) \in T.
+Proof.
+  induction t; intros; inversion H; subst; clear H; try solve [econstructor; eauto]; simpl.
+
+  apply T_Var. destruct (leb) eqn:IH. apply Nat.leb_le in IH.
+  generalize dependent g. generalize dependent T. generalize dependent n.
+  induction g1; simpl; intros; eauto. rewrite appGetbind. apply H2.
+  destruct n. inversion IH. simpl.
+  apply le_S_n in IH. simpl in H2. eapply IHg1 in IH; eauto.
+
+  apply Nat.leb_gt in IH. eapply length1_Some in IH. apply IH. apply H2.
+
+  apply T_Abs.
+  assert (S (length g1) = length (typ :: g1)). reflexivity.
+  rewrite H. apply IHt with (g1:= (typ :: g1)). apply H5.
+Qed.
+
+Lemma gb_lt_add : forall ctx ctx' p T n,
+  getbinding (S n) (ctx' ++ p :: ctx) = Some T ->
+  length ctx' < S n ->
+  getbinding n (ctx' ++ ctx) = Some T.
+Proof.
+  induction ctx'; simpl; intros; eauto.
+  destruct n. inversion H0; subst. apply Nat.leb_le in H2; inversion H2.
+  apply IHctx' in H. simpl. apply H. apply lt_S_n. apply H0.
+Qed.
+
+Lemma L9_3_8: forall t s Ts T ctx ctx',
+    (ctx' ++ Ts :: ctx) |- t \in T ->
+    ctx |- s \in Ts ->
+    (ctx' ++ ctx) |- subst (length ctx') s t \in T.
+Proof.
+  induction t; intros; inversion H; subst; clear H; try solve [econstructor; eauto]; simpl.
+  destruct eqb eqn:IHeq.
+  apply Nat.eqb_eq in IHeq; subst. apply shifting with (g2 := ctx') (g1:= []) in H0; simpl in H0.
+  rewrite <- (plus_O_n (length ctx')) in H3. rewrite (appGetbind ctx' ( (Ts) :: ctx) 0) in H3.
+  simpl in H3. inversion H3; subst. apply H0.
+  destruct ltb eqn:IHlt. apply Nat.ltb_lt in IHlt.
+  destruct n. inversion IHlt. simpl. apply T_Var. clear H0.
+  eapply gb_lt_add in H3; eauto.
+
+  apply Nat.ltb_ge in IHlt. apply T_Var.
+  apply le_lt_or_eq in IHlt. destruct IHlt.
+  eapply length1_Some in H; eauto.
+  subst. rewrite Nat.eqb_refl in IHeq; inversion IHeq.
+
+  apply T_Abs. apply (IHt s Ts T2 ctx ((typ) :: ctx')) in H6. simpl in H6. apply H6.
+  apply H0.
+Qed.
+
+Theorem T9_3_9 : forall t t' T ctx,
+    ctx |- t \in T ->
+    t --> t' ->
+    ctx |- t' \in T.
+Proof.
+  intros. generalize dependent T. induction H0; subst; simpl; intros; try solve [inversion H; subst; eauto].
+  -
+    inversion H; subst. apply IHstep in H5. apply T_If; auto.
+  -
+    inversion H; subst. apply IHstep in H4. apply T_App with T11; auto.
+  -
+    inversion H1; subst. apply IHstep in H7. apply T_App with T11; auto.
+  -
+    inversion H0; subst. clear H0. inversion H4; subst.
+    apply (L9_3_8 t12 t2 T11 T ctx []) in H2; eauto.
+Qed.
+
